\documentclass{article}
\begin{document}

\title{Integration Practice (Solutions)}
\date{\today}
\maketitle

Evaluate the following indefinite integrals:

\begin{enumerate}
\item $\int (3x^2 - 8x + 5) \, dx = x^3 - 4x^2 + 5x + C$ 
\item $\int (x^4 - 2x^3 + 7) \, dx = \frac{1}{5}x^5 - \frac{1}{2}x^4 + 7x + C$ 
\item $\int (\frac{1}{2}x^3 - \frac{3}{4}x^2 + x - 2) \, dx = \frac{1}{8}x^4 - \frac{1}{4}x^3 + \frac{1}{2}x^2 - 2x + C$ 
\item $\int (12x^5 - 5x^4 + 8x^3 - 2) \, dx = 2x^6 - x^5 + 2x^4 - 2x + C$  
\item $\int (9x^2 + 4x - 11) \, dx = 3x^3 + 2x^2 - 11x + C$ 
\item $\int (x^6 - 3x^4 + x^2 - 5) \, dx = \frac{1}{7}x^7 - \frac{3}{5}x^5 + \frac{1}{3}x^3 - 5x + C$  
\item $\int (5x^4 + 2x^2 - 9) \, dx = x^5 + \frac{2}{3}x^3 - 9x + C$
\item $\int (x^3 - 7x + 4) \, dx = \frac{1}{4}x^4 - \frac{7}{2}x^2 + 4x + C$
\item $\int (10x^5 - 3x^2 + 1) \, dx = \frac{5}{3}x^6 - x^3 + x + C$
\item $\int 3x^2 (x^3 + 2)^4 \, dx = \frac{1}{5}(x^3 + 2)^5 + C$ 
\item $\int 2x \sqrt{x^2 - 5} \, dx = \frac{2}{3}(x^2 - 5)^{3/2} + C$ 
\item $\int \cos(x) \sin^2(x) \, dx = \frac{1}{3}\sin^3(x) + C$ 
\item $\int  (2x + 1)(x^2 + x)^3 \, dx = \frac{1}{4}(x^2 + x)^4 + C$
\item $\int 4x^3 \sqrt[3]{x^4 + 1} \, dx = \frac{3}{4}(x^4 + 1)^{4/3} + C$
\end{enumerate}

\end{document}