\documentclass{article}
\begin{document}

\title{Session 8: Differentiation Practice - Logarithmic Functions}
\date{\today}
\maketitle

Differentiate the following functions:

\begin{enumerate}
\item $y = 10^x$

    $\frac{dy}{dx} = 10^x \ln(10)$

\item $y = 2^{x^2 + 3x}$

    $\frac{dy}{dx} = 2^{x^2 + 3x} \ln(2) \cdot (2x + 3)$

\item $y = 5^{\sin(x)}$

    $\frac{dy}{dx} = 5^{\sin(x)} \ln(5) \cdot \cos(x)$

\item $y = e^{2x} + 10^{3x}$

    $\frac{dy}{dx} = 2e^{2x} + 3 \cdot 10^{3x} \ln(10)$

\item $y = x^2 \cdot 3^x$

    $\frac{dy}{dx} = 2x \cdot 3^x + x^2 \cdot 3^x \ln(3)$

\item $y = \frac{2^x}{x + 1}$

    $\frac{dy}{dx} = \frac{2^x \ln(2) \cdot (x+1) - 2^x}{(x+1)^2}$

\item $y = 7^{\sqrt{x^2 + 1}}$

    $\frac{dy}{dx} = 7^{\sqrt{x^2 + 1}} \ln(7) \cdot \frac{x}{\sqrt{x^2 + 1}}$

\item $y = \log_{10}(2^x)$

    $\frac{dy}{dx} = \frac{1}{2^x \ln(10)} \cdot 2^x \ln(2) = \frac{\ln(2)}{\ln(10)}$

\item $y = 3^{x^3 + 2x} \cdot 5^{x^2 - 1}$

    $\frac{dy}{dx} = 3^{x^3 + 2x} \ln(3) \cdot (3x^2 + 2) \cdot 5^{x^2 - 1} + 3^{x^3 + 2x} \cdot 5^{x^2 - 1} \ln(5) \cdot 2x$

\item $y = (\sin(x))^{2^x}$ (Hint: Use logarithmic differentiation)

    $\ln(y) = 2^x \ln(\sin(x))$

    $\frac{1}{y} \frac{dy}{dx} = 2^x \ln(2) \ln(\sin(x)) + 2^x \cdot \frac{\cos(x)}{\sin(x)}$

    $\frac{dy}{dx} = (\sin(x))^{2^x} \left[ 2^x \ln(2) \ln(\sin(x)) + 2^x \cot(x) \right]$


\item $y = \ln(x^2 + 1)$

    $\frac{dy}{dx} = \frac{2x}{x^2 + 1}$

\item $y = \log_2(5x^3 - 2x)$

    $\frac{dy}{dx} = \frac{1}{(5x^3 - 2x) \ln(2)} \cdot (15x^2 - 2)$

\item $y = x^2 \ln(x)$

    $\frac{dy}{dx} = 2x \ln(x) + x^2 \cdot \frac{1}{x} = 2x \ln(x) + x$

\item $y = \frac{\ln(x)}{x + 1}$

    $\frac{dy}{dx} = \frac{\frac{1}{x} \cdot (x+1) - \ln(x)}{(x+1)^2} = \frac{x + 1 - x \ln(x)}{x(x+1)^2}$

\item $y = \ln(\sin(x))$

    $\frac{dy}{dx} = \frac{1}{\sin(x)} \cdot \cos(x) = \cot(x)$

\item $y = \ln(\sqrt{x^2 + 4})$

    $\frac{dy}{dx} = \frac{1}{\sqrt{x^2 + 4}} \cdot \frac{x}{\sqrt{x^2 + 4}} = \frac{x}{x^2 + 4}$

\item $y = e^x \ln(x)$

    $\frac{dy}{dx} = e^x \ln(x) + e^x \cdot \frac{1}{x} = e^x \left( \ln(x) + \frac{1}{x} \right)$

\item $y = \ln(x^3 + 3x^2 + 3x + 1)$ 

    $\frac{dy}{dx} = \frac{3x^2 + 6x + 3}{x^3 + 3x^2 + 3x + 1} = \frac{3(x+1)^2}{(x+1)^3} = \frac{3}{x+1}$

\item $y = \ln(\sec(x) + \tan(x))$

    $\frac{dy}{dx} = \frac{1}{\sec(x) + \tan(x)} \cdot (\sec(x) \tan(x) + \sec^2(x)) = \sec(x)$

\item $y = \ln|\ln(x)|$

    $\frac{dy}{dx} = \frac{1}{\ln(x)} \cdot \frac{1}{x} = \frac{1}{x \ln(x)}$

\item $y = \sqrt{\ln(x)}$

    $\frac{dy}{dx} = \frac{1}{2 \sqrt{\ln(x)}} \cdot \frac{1}{x} = \frac{1}{2x \sqrt{\ln(x)}}$

\item $y = \ln(\arctan(x))$

    $\frac{dy}{dx} = \frac{1}{\arctan(x)} \cdot \frac{1}{1+x^2} = \frac{1}{(1+x^2)\arctan(x)}$

\item $y = x \ln(x) - x$

    $\frac{dy}{dx} = \ln(x) + x \cdot \frac{1}{x} - 1 = \ln(x)$

\item $y = \ln(x^2 + 2x + 1)$

    $\frac{dy}{dx} = \frac{2x + 2}{x^2 + 2x + 1} = \frac{2(x+1)}{(x+1)^2} = \frac{2}{x+1}$

\item $y = [\ln(x)]^{\sin(x)}$ (Hint: Use logarithmic differentiation)

    $\ln(y) = \sin(x) \ln(\ln(x))$

    $\frac{1}{y} \frac{dy}{dx} = \cos(x) \ln(\ln(x)) + \sin(x) \cdot \frac{1}{\ln(x)} \cdot \frac{1}{x}$

    $\frac{dy}{dx} = [\ln(x)]^{\sin(x)} \left[ \cos(x) \ln(\ln(x)) + \frac{\sin(x)}{x \ln(x)} \right]$
\end{enumerate}

\end{document}